Finish adequacy TC enclave

theories/examples/enclaves/attestation_adequacy_template.v
@@ -7,8 +7,8 @@ From cap_machine Require Import
   stdpp_extra iris_extra
   rules logrel fundamental.
 From cap_machine.examples Require Import addr_reg_sample.
-(* From cap_machine.proofmode Require Export disjoint_regions_tactics. *)
 From cap_machine.proofmode Require Export mkregion_helpers disjoint_regions_tactics.
+From cap_machine Require Import assert.
 
 Definition register_to_lregister (reg : Reg) ( v : Version ) : LReg :=
   fmap (fun w => word_to_lword w v) reg.
@@ -29,8 +29,14 @@ Definition prog_region (P: prog): gmap Addr Word :=
   mkregion (prog_start P) (prog_end P) (prog_instrs P).
 
 
-Definition adv_condition adv w v :=
-  is_z w = true \/ in_region (word_to_lword w v) (prog_start adv) (prog_end adv) v.
+Definition in_region (w : Word) (b e : Addr) :=
+  match w with
+  | WCap p b' e' a => PermFlows RO p /\ (b <= b')%a /\ (e' <= e)%a
+  | _ => False
+  end.
+
+Definition adv_condition adv w :=
+  is_z w = true \/ in_region w (prog_start adv) (prog_end adv).
 
 Program Definition empty_prog a : prog := MkProg a a [] _.
 Next Obligation.
@@ -176,6 +182,21 @@ Proof.
   rewrite /memory_to_lmemory.
   apply map_disjoint_kmap; first by intros x y ?; simplify_eq.
   by apply map_disjoint_fmap.
+Qed.
+
+Lemma memory_to_lmemory_mk_logical_region_map la ws v:
+  memory_to_lmemory (list_to_map (zip la ws)) v
+  = logical_region_map la ((λ w : Word, word_to_lword w v) <$> ws) v.
+Proof.
+  revert la ws.
+  induction la as [|a la]; intros ws ; cbn in *.
+  - rewrite /memory_to_lmemory.
+    by rewrite fmap_empty kmap_empty.
+  - destruct ws as [|w ws]; cbn.
+    + rewrite /memory_to_lmemory.
+      by rewrite fmap_empty kmap_empty.
+    + rewrite memory_to_lmemory_insert.
+      by rewrite IHla.
 Qed.
 
 Lemma register_to_lregister_delete (reg : Reg) (r : RegName) (v : Version) :
@@ -375,91 +396,72 @@ End AdequacyInit.
 
 
 
-Record lib_entry := MkLibEntry {
-  lib_start : Addr;
-  lib_end : Addr;
-  lib_entrypoint : Addr;
-  lib_full_content : gmap Addr Word
+Record assert_library `{MachineParameters} := MkAssertLibrary {
+  (* assert library *)
+  assert_start : Addr;
+  assert_cap : Addr;
+  assert_flag : Addr;
+  assert_end : Addr;
+
+  assert_code_size :
+    (assert_start + length assert_subroutine_instrs)%a = Some assert_cap;
+  assert_cap_size :
+    (assert_cap + 1)%a = Some assert_flag;
+  assert_flag_size :
+    (assert_flag + 1)%a = Some assert_end;
 }.
 
-Definition entry_points (l: list lib_entry) : list Word :=
-  (map (λ entry, WCap E (lib_start entry) (lib_end entry) (lib_entrypoint entry)) l).
+Definition assert_library_content `{MachineParameters} (assert_layout : assert_library) : gmap Addr Word :=
+  (* code for the assert subroutine, followed by a capability to the assert flag
+     and the flag itself, initialized to 0. *)
+  mkregion (assert_start assert_layout) (assert_cap assert_layout) (lword_get_word <$> assert_subroutine_instrs)
+  ∪ list_to_map [(assert_cap assert_layout, WCap RW (assert_flag assert_layout) (assert_end assert_layout) (assert_flag assert_layout))]
+  ∪ list_to_map [(assert_flag assert_layout, WInt 0)] (* assert flag *).
 
-Record lib := MkLib {
-  pub_libs : list lib_entry;
-  priv_libs : list lib_entry
-}.
+Definition assert_entry_point `{MachineParameters} (assert_layout : assert_library) :=
+  WCap E (assert_start assert_layout) (assert_end assert_layout) (assert_start assert_layout).
 
-Record tbl {p : prog} {l : list lib_entry} := MkTbl {
-  prog_lower_bound : Addr ;
+Definition OK_invariant `{MachineParameters} (assert_layout : assert_library) (m : gmap Addr Word) : Prop :=
+  ∀ w, m !! (assert_flag assert_layout) = Some w → w = WInt 0%Z.
+
+Definition OK_dom `{MachineParameters} (assert_layout : assert_library) : gset Addr := {[ assert_flag assert_layout ]}.
+
+Program Definition OK_dom_correct `{MachineParameters} (assert_layout : assert_library) :
+  ∀ m m',
+    (∀ a, a ∈ OK_dom assert_layout → ∃ x, m !! a = Some x ∧ m' !! a = Some x) →
+    OK_invariant assert_layout m ↔ OK_invariant assert_layout m'.
+Proof.
+  intros m m' Hdom.
+  destruct Hdom with (assert_flag assert_layout) as [w [Hw1 Hw2] ]. rewrite /OK_dom. set_solver.
+  split;intros HOK;intros w' Hw';simplify_eq;apply HOK;auto.
+Defined.
+
+Definition adequacy_flag_inv `{MachineParameters} (assert_layout : assert_library) : memory_inv :=
+  {| minv := OK_invariant assert_layout;
+     minv_dom := {[ assert_flag assert_layout ]} ;
+     minv_dom_correct := OK_dom_correct assert_layout |}.
+
+Record assert_tbl := MkTbl {
   tbl_start : Addr ;
   tbl_end : Addr ;
-  tbl_size : (tbl_start + length l)%a = Some tbl_end ;
-  tbl_prog_link : (prog_lower_bound + 1)%a = Some (prog_start p) ;
-
-  tbl_disj : mkregion tbl_start tbl_end (entry_points l) ##ₘ
-             mkregion prog_lower_bound (prog_end p) ((WCap RO tbl_start tbl_end tbl_start) :: (prog_instrs p))
+  tbl_size : (tbl_start + 1)%a = Some tbl_end ;
 }.
 
-Definition tbl_region {p l} (t : @tbl p l) : gmap Addr Word :=
-  mkregion (tbl_start t) (tbl_end t) (entry_points l).
-Definition prog_lower_bound_region {l} (p : prog) (t : @tbl p l) : gmap Addr Word :=
-  mkregion (prog_lower_bound t) (prog_end p) ((WCap RO (tbl_start t) (tbl_end t) (tbl_start t)) :: (prog_instrs p)).
-Definition prog_tbl_region {l} (p : prog) (t : @tbl p l) : gmap Addr Word :=
-  prog_lower_bound_region p t ∪ tbl_region t.
-Definition prog_tbl_data_region {l} (p data: prog) (t : @tbl p l) : gmap Addr Word :=
-  prog_lower_bound_region p t ∪ tbl_region t ∪ prog_region data.
+Definition assert_tbl_region `{MachineParameters} (tbl : assert_tbl) (assert_layout : assert_library) : gmap Addr Word :=
+  mkregion (tbl_start tbl) (tbl_end tbl) [assert_entry_point assert_layout].
 
-Lemma prog_lower_bound_region_cons {l} (p : prog) (t : @tbl p l) :
-  prog_lower_bound_region p t = <[(prog_lower_bound t):=WCap RO (tbl_start t) (tbl_end t) (tbl_start t)]> (prog_region p)
-  ∧ (prog_region p) !! (prog_lower_bound t) = None.
-Proof.
-  rewrite /prog_lower_bound_region /mkregion.
-  pose proof (tbl_prog_link t) as Ht.
-  destruct (decide (prog_start p = prog_end p)).
-  - rewrite e in Ht. rewrite /prog_region /mkregion finz_seq_between_singleton// e finz_seq_between_empty /=.
-    split;auto. solve_addr.
-  - pose proof (prog_size p).
-    assert (prog_start p <= prog_end p)%a.
-    { solve_addr. }
-    rewrite (finz_seq_between_cons (prog_lower_bound t));[|solve_addr].
-    simpl. rewrite (addr_incr_eq Ht) /=. split;auto.
-    rewrite /prog_region /mkregion.
-    apply not_elem_of_list_to_map.
-    rewrite fst_zip. apply not_elem_of_finz_seq_between. solve_addr.
-    rewrite finz_seq_between_length /finz.dist. solve_addr.
-Qed.
-
-Fixpoint lib_region (l : list lib_entry) : gmap Addr Word :=
-  match l with
-  | [] => ∅
-  | e :: l => (lib_full_content e) ∪ (lib_region l)
-  end.
-
-Lemma lib_region_app l1 l2 :
-  lib_region (l1 ++ l2) = lib_region l1 ∪ lib_region l2.
-Proof.
-  induction l1. by rewrite app_nil_l map_empty_union.
-  by rewrite /= IHl1 map_union_assoc.
-Qed.
-
-Definition tbl_pub (p : prog) (l : lib) := @tbl p (pub_libs l).
-Definition tbl_priv (p : prog) (l : lib) := @tbl p ((pub_libs l) ++ (priv_libs l)).
-
-Module with_adv_and_link.
-
-
-Definition is_initial_registers
-  (P Adv: prog) (Lib : lib) (P_tbl : tbl_priv P Lib) (Adv_tbl : tbl_pub Adv Lib) (reg: gmap RegName Word) (r_adv: RegName) :=
-  reg !! PC = Some (WCap RWX (prog_lower_bound P_tbl) (prog_end P) (prog_start P)) ∧
-  reg !! r_adv = Some (WCap RWX (prog_lower_bound Adv_tbl) (prog_end Adv) (prog_start Adv)) ∧
+Definition is_initial_registers `{MachineParameters}
+  (P Adv: prog) (AssertLib : assert_library) (tbl : assert_tbl) (regs: Reg) (r_adv: RegName):=
+  regs !! PC = Some (WCap RWX (prog_start P) (prog_end P) (prog_start P)) ∧
+  regs !! r_adv = Some (WCap RWX (prog_start Adv) (prog_end Adv) (prog_start Adv)) ∧
   PC ≠ r_adv ∧
   (∀ (r: RegName), r ∉ ({[ PC ; r_adv ]} : gset RegName) →
-     ∃ (w:Word), reg !! r = Some w ∧ is_z w = true).
+     ∃ (w:Word), regs !! r = Some w ∧ is_z w = true).
 
-Lemma initial_registers_full_map (P Adv: prog) (Lib : lib) (P_tbl : tbl_priv P Lib) (Adv_tbl : tbl_pub Adv Lib) reg r_adv :
-  is_initial_registers P Adv Lib P_tbl Adv_tbl reg r_adv →
-  (∀ r, is_Some (reg !! r)).
+Lemma initial_registers_full_map `{MachineParameters}
+  (P Adv: prog) (AssertLib : assert_library) (tbl : assert_tbl) (regs: Reg) (r_adv : RegName) :
+  is_initial_registers P Adv AssertLib tbl regs r_adv →
+  (∀ r, is_Some (regs !! r)).
 Proof.
   intros (HPC & Hr0 & Hne & Hothers) r.
   destruct (decide (r = PC)) as [->|]. by eauto.
@@ -467,21 +469,46 @@ Proof.
   destruct (Hothers r) as (w & ? & ?); [| eauto]. set_solver.
 Qed.
 
-Definition is_initial_memory (P Adv: prog) (Lib : lib) (P_tbl : tbl_priv P Lib) (Adv_tbl : tbl_pub Adv Lib) (m: gmap Addr Word) :=
-  prog_tbl_region P P_tbl ⊆ m
-  ∧ prog_tbl_region Adv Adv_tbl ⊆ m
-  ∧ lib_region ((pub_libs Lib) ++ (priv_libs Lib)) ⊆ m
-  ∧ prog_tbl_region P P_tbl ##ₘ prog_tbl_region Adv Adv_tbl
-  ∧ prog_tbl_region P P_tbl ##ₘ lib_region ((pub_libs Lib) ++ (priv_libs Lib))
-  ∧ prog_tbl_region Adv Adv_tbl ##ₘ lib_region ((pub_libs Lib) ++ (priv_libs Lib))
-  ∧ lib_region (pub_libs Lib) ##ₘ lib_region (priv_libs Lib).
+Definition is_initial_memory `{MachineParameters}
+  (P Adv: prog) (AssertLib : assert_library) (tbl : assert_tbl) (m: Mem) :=
+  prog_region P ⊆ m
+  ∧ prog_region Adv ⊆ m
+  ∧ assert_tbl_region tbl AssertLib ⊆ m
+  ∧ (assert_library_content AssertLib) ⊆ m
+  ∧ prog_region P ##ₘ prog_region Adv
+  ∧ prog_region P ##ₘ assert_tbl_region tbl AssertLib
+  ∧ prog_region P ##ₘ (assert_library_content AssertLib)
+  ∧ prog_region Adv ##ₘ assert_tbl_region tbl AssertLib
+  ∧ prog_region Adv ##ₘ (assert_library_content AssertLib)
+  ∧ assert_tbl_region tbl AssertLib ##ₘ (assert_library_content AssertLib).
 
-Definition initial_memory_domain (P Adv: prog) (Lib : lib) (P_tbl : tbl_priv P Lib) (Adv_tbl : tbl_pub Adv Lib) : gset Addr :=
-  dom (prog_tbl_region P P_tbl)
-      ∪ dom (prog_tbl_region Adv Adv_tbl)
-      ∪ dom (lib_region ((pub_libs Lib) ++ (priv_libs Lib))).
+Lemma adequacy_flag_inv_is_initial_memory `{MachineParameters}
+  (P Adv: prog) (AssertLib : assert_library) (tbl : assert_tbl) (m : Mem) :
+  is_initial_memory P Adv AssertLib tbl m →
+  minv (adequacy_flag_inv AssertLib) m.
+Proof.
+  intros Hinit. intros a Hin.
+  destruct Hinit as (?&?&Hlibs&?&?&?&Hlibdisj).
+  cbn in Hlibs.
+  pose proof (assert_code_size AssertLib). pose proof (assert_cap_size AssertLib).
+  pose proof (assert_flag_size AssertLib).
+  assert (list_to_map [(assert_flag AssertLib, WInt 0)] ⊆ m) as Hassert_flag.
+  { etrans;[|eauto]. eapply map_union_subseteq_r'. 2: done.
+    disjoint_map_to_list.
+    apply elem_of_disjoint. intro. rewrite elem_of_app !elem_of_finz_seq_between !elem_of_list_singleton.
+    intros [ [? ?]|?] ->; solve_addr. }
+  eapply (lookup_weaken _ _ (assert_flag AssertLib) (WInt 0)) in Hassert_flag.
+    by simplify_eq. by simplify_map_eq.
+Qed.
 
-(* NOTE: solely this version of adequacy has been updated to work with seals, by having allocated seals in the precondition *)
+Local Instance reserved_addresses_assert `{MachineParameters} (layout : assert_library) (vinit : Version) : ReservedAddresses.
+Proof. apply (ReservedAddressesG [assert_flag layout] vinit). Defined.
+
+Definition assertInv `{ceriseG Σ, logrel_na_invs Σ, MachineParameters} (layout : assert_library) :=
+  assert.assert_inv (assert_start layout) (assert_flag layout) (assert_end layout).
+
+Definition assertN : namespace := nroot .@ "assert".
+
 Section Adequacy.
   Context (Σ: gFunctors).
   Context {inv_preg: invGpreS Σ}.
@@ -495,10 +522,8 @@ Section Adequacy.
   Context `{MP: MachineParameters}.
 
   Context (P Adv: prog).
-  Context (Lib : lib).
-  Context (P_tbl : @tbl_priv P Lib).
-  Context (Adv_tbl : @tbl_pub Adv Lib).
-  Context (I : memory_inv).
+  Context (AssertLib : assert_library).
+  Context (tbl_assert_tbl : assert_tbl).
   Context (r_adv : RegName).
   Context (vinit : Version).
 
@@ -509,51 +534,49 @@ Section Adequacy.
     (etbl' : ETable) (ecur' : ENum)
     (es: list cap_lang.expr)
     :
-    is_initial_memory P Adv Lib P_tbl Adv_tbl m →
+    let I := (adequacy_flag_inv AssertLib) in
+    let RA := reserved_addresses_assert AssertLib vinit in
+
+    is_initial_memory P Adv AssertLib tbl_assert_tbl m →
     is_complete_memory m →
-    is_initial_registers P Adv Lib P_tbl Adv_tbl reg r_adv →
+    is_initial_registers P Adv AssertLib tbl_assert_tbl reg r_adv →
     is_complete_registers reg m →
 
-    Forall (fun w => adv_condition Adv w vinit) (prog_instrs Adv) →
+    Forall (fun w => adv_condition Adv w) (prog_instrs Adv) →
     minv I m →
-    minv_dom I ⊆ dom (lib_region (priv_libs Lib)) →
 
     let filtered_map := λ (m : gmap Addr Word), filter (fun '(a, _) => a ∉ minv_dom I) m in
-    (∀ `{ceriseG Σ, sealStoreG Σ, NA: logrel_na_invs Σ, ReservedAddresses, subG Σ' Σ} rmap,
+    (∀ `{ceriseG Σ, sealStoreG Σ, NA: logrel_na_invs Σ, subG Σ' Σ} rmap,
         dom rmap = all_registers_s ∖ {[ PC; r_adv ]} →
      ⊢ inv invN (minv_sep I vinit)
      (* ∗ custom_enclave_inv *)
        ∗ @na_own _ (@logrel_na_invG _ NA) logrel_nais ⊤ (*XXX*)
+        ∗ @na_inv _ _ _ (@logrel_na_invG _ NA) logrel_nais assertN (assertInv AssertLib vinit)
 
        (* Registers *)
-       ∗ PC ↦ᵣ LCap RWX (prog_lower_bound P_tbl) (prog_end P) (prog_start P) vinit
-       ∗ r_adv ↦ᵣ LCap RWX (prog_lower_bound Adv_tbl) (prog_end Adv) (prog_start Adv) vinit
+       ∗ PC ↦ᵣ LCap RWX (prog_start P) (prog_end P) (prog_start P) vinit
+       ∗ r_adv ↦ᵣ LCap RWX (prog_start Adv) (prog_end Adv) (prog_start Adv) vinit
        ∗ ([∗ map] r↦w ∈ (register_to_lregister rmap vinit), r ↦ᵣ w ∗ ⌜is_zL w = true⌝)
 
        (* Memory *)
-       (* P program and table *)
-       ∗ (prog_lower_bound P_tbl, vinit) ↦ₐ (LCap RO (tbl_start P_tbl) (tbl_end P_tbl) (tbl_start P_tbl) vinit)
-       ∗ ([∗ map] a↦w ∈ (memory_to_lmemory (tbl_region P_tbl) vinit), a ↦ₐ w)
+       (* P program *)
        ∗ ([∗ map] a↦w ∈ (memory_to_lmemory (prog_region P) vinit), a ↦ₐ w)
-       (* Adv program and table *)
-       ∗ (prog_lower_bound Adv_tbl, vinit) ↦ₐ (LCap RO (tbl_start Adv_tbl) (tbl_end Adv_tbl) (tbl_start Adv_tbl) vinit)
-       ∗ ([∗ map] a↦w ∈ (memory_to_lmemory (tbl_region Adv_tbl) vinit), a ↦ₐ w)
+       (* Adv program  *)
        ∗ ([∗ map] a↦w ∈ (memory_to_lmemory (prog_region Adv) vinit), a ↦ₐ w)
-       (* filtered entries *)
-       ∗ ([∗ map] a↦w ∈ (memory_to_lmemory (lib_region (pub_libs Lib)) vinit), a ↦ₐ w)
-       ∗ ([∗ map] a↦w ∈ (memory_to_lmemory (filtered_map (lib_region (priv_libs Lib))) vinit), a ↦ₐ w)
+       (* Linking Table *)
+       ∗ ([∗ map] a↦w ∈ (memory_to_lmemory (assert_tbl_region tbl_assert_tbl AssertLib) vinit), a ↦ₐ w)
 
-       ∗ EC⤇ 0
+       ∗ EC⤇ 0%nat
        ∗ ([∗ set] o ∈ gset_all_otypes, can_alloc_pred o)
 
        -∗ WP Seq (Instr Executable) {{ λ _, True }}) →
 
     rtc erased_step
-      ([Seq (Instr Executable)] , {| reg := reg ; mem := m ; etable := ∅ ; enumcur := 0 |})
+      ([Seq (Instr Executable)] , {| reg := reg ; mem := m ; etable := ∅ ; enumcur := 0%nat |})
       (es, {| reg := reg' ; mem := m' ; etable := etbl' ; enumcur := ecur' |}) →
     minv I m'.
   Proof.
-    intros Hm Hm_complete Hreg Hreg_complete Hadv HI HIdom prog_map Hspec Hstep.
+    intros I RA Hm Hm_complete Hreg Hreg_complete Hadv HI prog_map Hspec Hstep.
     pose proof (@wp_invariance Σ cap_lang _ NotStuck) as WPI. cbn in WPI.
     pose (fun (c:ExecConf) => minv I c.(mem)) as state_is_good.
     specialize (WPI
@@ -589,70 +612,123 @@ Section Adequacy.
                       enclave_agree_preg enclave_excl_preg γhist γprev γlive
                       EC_preg γEC.
     set ( addr_inv := (elements (minv_dom I))).
-    pose reservedaddresses := ReservedAddressesG addr_inv vinit.
-    specialize (Hspec ceriseg seal_storeg logrel_na_invs reservedaddresses).
-    destruct Hm as (HM & HA & HL & (Hdisj1 & Hdisj2 & Hdisj3 & Hdisj4)).
+    (* pose reservedaddresses := ReservedAddressesG addr_inv vinit. *)
+    specialize (Hspec ceriseg seal_storeg logrel_na_invs).
+    destruct Hm as (HProg & HAdv & HLink & HAssert & (Hdisj1 & Hdisj2 & Hdisj3 & Hdisj4 & Hdisj5 & Hdisj6)).
 
     iDestruct (big_sepM_subseteq with "Hmem") as "Hprogadv".
     { transitivity (
           (memory_to_lmemory (
-          prog_tbl_region P P_tbl ∪
-                    prog_tbl_region Adv Adv_tbl ∪
-                    lib_region ((pub_libs Lib) ++ (priv_libs Lib))) vinit)
+               prog_region P ∪
+                 prog_region Adv ∪
+                 ( assert_tbl_region tbl_assert_tbl AssertLib ) ∪
+                 assert_library_content AssertLib)
+             vinit)
         ); eauto.
       apply memory_to_lmemory_subseteq.
       rewrite map_subseteq_spec. intros * HH.
-      apply lookup_union_Some in HH; auto. destruct HH as [HH|HH].
-      apply lookup_union_Some in HH; auto. destruct HH as [HH|HH].
-      eapply map_subseteq_spec in HM; eauto.
-      eapply map_subseteq_spec in HA; eauto.
-      eapply map_subseteq_spec in HL; eauto.
-      apply map_disjoint_union_l;auto.
+      apply lookup_union_Some in HH; auto.
+      2:{
+        apply map_disjoint_union_l;auto.
+        split; auto.
+        apply map_disjoint_union_l;auto.
+      }
+      destruct HH as [HH|HH].
+      - apply lookup_union_Some in HH; auto.
+        2:{ apply map_disjoint_union_l;auto. }
+        destruct HH as [HH|HH].
+        + apply lookup_union_Some in HH; auto.
+          destruct HH as [HH|HH].
+          * eapply map_subseteq_spec in HProg; eauto.
+          * eapply map_subseteq_spec in HAdv; eauto.
+        + eapply map_subseteq_spec in HLink; eauto.
+      - eapply map_subseteq_spec in HAssert; eauto.
     }
-    iEval (rewrite 2!memory_to_lmemory_union) in "Hprogadv".
-    iDestruct (big_sepM_union with "Hprogadv") as "[Hprog Hlib]";
-      [apply map_disjoint_union_l;auto;split;apply memory_to_lmemory_disjoint; auto|].
+    iEval (rewrite 3!memory_to_lmemory_union) in "Hprogadv".
+    iDestruct (big_sepM_union with "Hprogadv") as "[Hprog HAssertLib]".
+    { apply map_disjoint_union_l;auto;split; last (apply memory_to_lmemory_disjoint; auto).
+      apply map_disjoint_union_l;auto;split; apply memory_to_lmemory_disjoint; auto.
+    }
+    iDestruct (big_sepM_union with "Hprog") as "[Hprog HLink]".
+    { apply map_disjoint_union_l;auto;split;apply memory_to_lmemory_disjoint; auto.
+    }
     iDestruct (big_sepM_union with "Hprog") as "[Hp Hadv]";
       [apply memory_to_lmemory_disjoint; auto|].
 
-    pose proof (tbl_disj P_tbl) as Hdisjtbl1.
-    pose proof (tbl_disj Adv_tbl) as Hdisjtbl2.
-    pose proof (tbl_prog_link P_tbl) as Hlink1.
-    pose proof (tbl_prog_link Adv_tbl) as Hlink2.
-
-    iEval (rewrite memory_to_lmemory_union) in "Hp".
-    iDestruct (big_sepM_union with "Hp") as "[Hp Hp_tbl]";
-      [apply memory_to_lmemory_disjoint; auto|].
-    iEval (rewrite memory_to_lmemory_union) in "Hadv".
-    iDestruct (big_sepM_union with "Hadv") as "[Hadv Hadv_tbl]";
-      [apply memory_to_lmemory_disjoint; auto|].
-
-    iEval (rewrite lib_region_app memory_to_lmemory_union) in "Hlib".
-    iDestruct (big_sepM_union with "Hlib") as "[Hlib_pub Hlib_priv]";
-      [apply memory_to_lmemory_disjoint; auto|].
-
-
     set prog_in_inv :=
-      filter (fun '(a, _) => a ∈ minv_dom I) (lib_region (priv_libs Lib)).
+      filter (fun '(a, _) => a ∈ minv_dom I) (assert_library_content AssertLib).
     set prog_nin_inv :=
-      filter (fun '(a, _) => a ∉ minv_dom I) (lib_region (priv_libs Lib)).
-    rewrite (_: lib_region (priv_libs Lib) = prog_in_inv ∪ prog_nin_inv).
+      filter (fun '(a, _) => a ∉ minv_dom I) (assert_library_content AssertLib).
+    rewrite (_: (assert_library_content AssertLib) = prog_in_inv ∪ prog_nin_inv).
     2: { symmetry. apply map_filter_union_complement. }
-    iEval (rewrite memory_to_lmemory_union) in "Hlib_priv".
-    iDestruct (big_sepM_union with "Hlib_priv") as "[Hlib_inv Hlib_priv]".
+    iEval (rewrite memory_to_lmemory_union) in "HAssertLib".
+    iDestruct (big_sepM_union with "HAssertLib") as "[Hassert_inv Hassert]".
     { by apply memory_to_lmemory_disjoint, map_disjoint_filter_complement. }
 
-    iMod (inv_alloc invN ⊤ (minv_sep I vinit) with "[Hlib_inv]") as "#Hinv".
+    iMod (inv_alloc invN ⊤ (minv_sep I vinit) with "[Hassert_inv]") as "#Hinv".
     { iNext. unfold minv_sep. iExists prog_in_inv. iFrame. iPureIntro.
-      assert (minv_dom I ⊆ dom (lib_region (priv_libs Lib))).
-      { etransitivity. eapply HIdom. auto. }
+      assert (minv_dom I ⊆ dom (assert_library_content AssertLib)).
+      { subst I.
+        rewrite /assert_library_content.
+        setoid_rewrite dom_union.
+        cbn.
+        rewrite dom_insert_L dom_empty_L union_empty_r_L.
+        apply union_subseteq_r.
+      }
       rewrite filter_dom_is_dom; auto. split; auto.
       eapply minv_sub_restrict; [ | | eapply HI]. rewrite filter_dom_is_dom//.
-      transitivity (lib_region (priv_libs Lib)); auto. rewrite /prog_in_inv.
-      eapply map_filter_subseteq; typeclasses eauto.
-      transitivity (lib_region (pub_libs Lib ++ priv_libs Lib)); auto.
-      rewrite lib_region_app. apply map_union_subseteq_r. auto.
+      transitivity (assert_library_content AssertLib); auto. rewrite /prog_in_inv.
+      eapply map_filter_subseteq;typeclasses eauto.
     }
+
+  iMod (@na_inv_alloc _ _ _ (@logrel_na_invG _ logrel_na_invs) logrel.logrel_nais ⊤ assertN (assertInv AssertLib vinit)
+          with "[Hassert]") as "#Hinv_assert".
+  { iNext. rewrite /assertInv /assert_inv /assert_library_content.
+    iExists (assert_cap AssertLib).
+    pose proof (assert_code_size AssertLib). pose proof (assert_cap_size AssertLib).
+    pose proof (assert_flag_size AssertLib).
+    rewrite /prog_nin_inv.
+    rewrite map_filter_union.
+    2: { disjoint_map_to_list. apply elem_of_disjoint. intro.
+         rewrite elem_of_app elem_of_finz_seq_between !elem_of_list_singleton.
+         intros [ [? ?]|?]; solve_addr. }
+    rewrite memory_to_lmemory_union.
+    iDestruct (big_sepM_union with "Hassert") as "[Hassert _]".
+    { apply memory_to_lmemory_disjoint.
+      eapply map_disjoint_filter. disjoint_map_to_list.
+      apply elem_of_disjoint. intro.
+      rewrite elem_of_app elem_of_finz_seq_between !elem_of_list_singleton.
+      intros [ [? ?]|?]; solve_addr. }
+    rewrite map_filter_id.
+    2: { intros ? ? HH%elem_of_dom_2. rewrite !dom_union_L dom_mkregion_eq in HH.
+         2: solve_addr. apply elem_of_union in HH.
+         rewrite elem_of_singleton. destruct HH as [HH|HH].
+         rewrite -> elem_of_list_to_set, elem_of_finz_seq_between in HH; solve_addr.
+         rewrite -> dom_list_to_map_singleton, elem_of_list_to_set, elem_of_list_singleton in HH; solve_addr. }
+    rewrite memory_to_lmemory_union.
+    iDestruct (big_sepM_union with "Hassert") as "[Hassert Hcap]".
+    { apply memory_to_lmemory_disjoint.
+      disjoint_map_to_list. apply elem_of_disjoint. intro.
+      rewrite elem_of_finz_seq_between !elem_of_list_singleton. solve_addr. }
+    (* subst vinit. *)
+    rewrite memory_to_lmemory_insert.
+    iEval (cbn) in "Hcap".
+    iDestruct (big_sepM_insert with "Hcap") as "[Hcap _]"; first done.
+    iFrame "Hcap".
+    iSplitL "Hassert"; cycle 1.
+    + iPureIntro. repeat split; solve_addr.
+    + iApply (mkregion_sepM_to_sepL2 with "[Hassert]"); auto.
+      { apply Forall_forall.
+        intros.
+        cbn in *.
+        repeat (rewrite elem_of_cons in H12; destruct H12 as [-> | H12]; first done).
+        set_solver+H3.
+      }
+      { solve_addr. }
+      rewrite (_: assert_cap AssertLib = assert_start AssertLib ^+ length assert_subroutine_instrs)%a. 2: solve_addr.
+    iFrame "Hassert".
+    }
+
 
     unfold is_initial_registers in Hreg.
     destruct Hreg as (HPC & Hr0 & Hne & Hrothers).
@@ -693,27 +769,14 @@ Section Adequacy.
     rewrite !register_to_lregister_delete.
     set rmap := (delete _ _) : Reg.
 
-    pose proof (prog_lower_bound_region_cons P P_tbl) as [HeqP HNoneP].
-    pose proof (prog_lower_bound_region_cons Adv Adv_tbl) as [HeqAdv HNoneAdv].
-    rewrite HeqP HeqAdv.
-
-    iEval (rewrite memory_to_lmemory_insert) in "Hp".
-    iDestruct (big_sepM_insert with "Hp") as "[Hlinkp Hp]"
-    ;[rewrite memory_to_lmemory_lookup;apply fmap_None; auto|].
-    iEval (rewrite memory_to_lmemory_insert) in "Hadv".
-    iDestruct (big_sepM_insert with "Hadv") as "[Hlinkadv Hadv]"
-    ;[rewrite memory_to_lmemory_lookup;apply fmap_None; auto|].
-
     iPoseProof (Hspec _ rmap with
                  "[$HPC $Hr0 $Hreg $HEC $Hseal_store
-                  $Hlinkp $Hp $Hlinkadv $Hadv $Hp_tbl
-                  $Hadv_tbl $Hlib_pub $Hlib_priv
+                  $Hp $Hadv $HLink $Hinv_assert
                   $Hinv $Hna]") as "Spec".
     { subst rmap. rewrite !dom_delete_L regmap_full_dom. set_solver+. apply Hreg_full. }
-
     iModIntro.
     iExists (fun σ κs _ => state_interp_logical σ).
-    iExists (fun _ => True)%I. cbn. iFrame.
+    iExists (fun _ => True)%I. iFrame.
     iSplitL.
     {
       iExists (register_to_lregister reg vinit),
@@ -739,277 +802,72 @@ Section Adequacy.
     unfold minv_sep. iDestruct "Hx" as (mi) "(Hmi & Hmi_dom & %)".
     iDestruct "Hmi_dom" as %Hmi_dom.
     iDestruct (gen_heap_valid_inclSepM with "Hmem' Hmi") as %Hmi_incl.
-    iModIntro. iPureIntro. rewrite /state_is_good //=.
+    iModIntro. iPureIntro.
+    rewrite /state_is_good.
     eapply minv_sub_extend; [| |eassumption].
     rewrite Hmi_dom //.
     destruct Hstate_inv.
     eapply state_phys_log_corresponds_memory_to_lmemory; eauto.
+    subst I.
+    subst RA.
+    rewrite /reserved_addresses /=.
+    apply elements_singleton.
   Qed.
 
 End Adequacy.
 
-  Lemma template_adequacy
-    `{MP: MachineParameters} (Σ : gFunctor)
-    (P Adv: prog) (Lib : lib)
-    (P_tbl : @tbl_priv P Lib)
-    (Adv_tbl : @tbl_pub Adv Lib) (I: memory_inv) (r_adv : RegName)
-    (m m': Mem) (reg reg': Reg) (etbl' : ETable) (ecur' : ENum)
-    (es: list cap_lang.expr):
-    let vinit := 0 in
+Lemma template_adequacy
+  `{MP: MachineParameters}
+  (Σ : gFunctors)
+  (P Adv: prog) (AssertLib : assert_library) (tbl_assert_tbl : assert_tbl)
+  (r_adv : RegName)
+  (m m': Mem) (reg reg': Reg)
+  (etbl' : ETable) (ecur' : ENum)
+  (es: list cap_lang.expr)
+  :
+  let I := (adequacy_flag_inv AssertLib) in
+  let vinit := 0%nat in
+  let RA := reserved_addresses_assert AssertLib vinit in
+  is_initial_memory P Adv AssertLib tbl_assert_tbl m →
+  is_complete_memory m →
+  is_initial_registers P Adv AssertLib tbl_assert_tbl reg r_adv →
+  is_complete_registers reg m →
 
-    is_initial_memory P Adv Lib P_tbl Adv_tbl m →
-    is_complete_memory m →
-    is_initial_registers P Adv Lib P_tbl Adv_tbl reg r_adv →
-    is_complete_registers reg m →
+  Forall (fun w => adv_condition Adv w) (prog_instrs Adv) →
+  minv I m →
 
-    Forall (fun w => adv_condition Adv w vinit) (prog_instrs Adv) →
-    minv I m →
-    minv_dom I ⊆ dom (lib_region (priv_libs Lib)) →
-
-    let filtered_map := λ (m : gmap Addr Word), filter (fun '(a, _) => a ∉ minv_dom I) m in
-    (∀ `{ceriseG Σ', sealStoreG Σ', NA: logrel_na_invs Σ', ReservedAddresses, subG Σ Σ'} rmap,
-        dom rmap = all_registers_s ∖ {[ PC; r_adv ]} →
+  let filtered_map := λ (m : gmap Addr Word), filter (fun '(a, _) => a ∉ minv_dom I) m in
+  (∀ `{ceriseG Σ', sealStoreG Σ', NA: logrel_na_invs Σ', subG Σ Σ'} rmap,
+     dom rmap = all_registers_s ∖ {[ PC; r_adv ]} →
      ⊢ inv invN (minv_sep I vinit)
-     (* ∗ custom_enclave_inv *)
-       ∗ @na_own _ (@logrel_na_invG _ NA) logrel_nais ⊤ (*XXX*)
+     ∗ na_own logrel_nais ⊤ (*XXX*)
+     ∗ na_inv logrel_nais assertN (assertInv AssertLib vinit)
 
-       (* Registers *)
-       ∗ PC ↦ᵣ LCap RWX (prog_lower_bound P_tbl) (prog_end P) (prog_start P) vinit
-       ∗ r_adv ↦ᵣ LCap RWX (prog_lower_bound Adv_tbl) (prog_end Adv) (prog_start Adv) vinit
-       ∗ ([∗ map] r↦w ∈ (register_to_lregister rmap vinit), r ↦ᵣ w ∗ ⌜is_zL w = true⌝)
+     (* Registers *)
+     ∗ PC ↦ᵣ LCap RWX (prog_start P) (prog_end P) (prog_start P) vinit
+     ∗ r_adv ↦ᵣ LCap RWX (prog_start Adv) (prog_end Adv) (prog_start Adv) vinit
+     ∗ ([∗ map] r↦w ∈ (register_to_lregister rmap vinit), r ↦ᵣ w ∗ ⌜is_zL w = true⌝)
 
-       (* Memory *)
-       (* P program and table *)
-       ∗ (prog_lower_bound P_tbl, vinit) ↦ₐ (LCap RO (tbl_start P_tbl) (tbl_end P_tbl) (tbl_start P_tbl) vinit)
-       ∗ ([∗ map] a↦w ∈ (memory_to_lmemory (tbl_region P_tbl) vinit), a ↦ₐ w)
-       ∗ ([∗ map] a↦w ∈ (memory_to_lmemory (prog_region P) vinit), a ↦ₐ w)
-       (* Adv program and table *)
-       ∗ (prog_lower_bound Adv_tbl, vinit) ↦ₐ (LCap RO (tbl_start Adv_tbl) (tbl_end Adv_tbl) (tbl_start Adv_tbl) vinit)
-       ∗ ([∗ map] a↦w ∈ (memory_to_lmemory (tbl_region Adv_tbl) vinit), a ↦ₐ w)
-       ∗ ([∗ map] a↦w ∈ (memory_to_lmemory (prog_region Adv) vinit), a ↦ₐ w)
-       (* filtered entries *)
-       ∗ ([∗ map] a↦w ∈ (memory_to_lmemory (lib_region (pub_libs Lib)) vinit), a ↦ₐ w)
-       ∗ ([∗ map] a↦w ∈ (memory_to_lmemory (filtered_map (lib_region (priv_libs Lib))) vinit), a ↦ₐ w)
+     (* Memory *)
+     (* P program *)
+     ∗ ([∗ map] a↦w ∈ (memory_to_lmemory (prog_region P) vinit), a ↦ₐ w)
+     (* Adv program  *)
+     ∗ ([∗ map] a↦w ∈ (memory_to_lmemory (prog_region Adv) vinit), a ↦ₐ w)
+     (* Linking Table *)
+     ∗ ([∗ map] a↦w ∈ (memory_to_lmemory (assert_tbl_region tbl_assert_tbl AssertLib) vinit), a ↦ₐ w)
 
-       ∗ EC⤇ 0
-       ∗ ([∗ set] o ∈ gset_all_otypes, can_alloc_pred o)
+     ∗ EC⤇ 0%nat
+     ∗ ([∗ set] o ∈ gset_all_otypes, can_alloc_pred o)
 
        -∗ WP Seq (Instr Executable) {{ λ _, True }}) →
 
-    rtc erased_step
-      ([Seq (Instr Executable)] , {| reg := reg ; mem := m ; etable := ∅ ; enumcur := 0 |})
-      (es, {| reg := reg' ; mem := m' ; etable := etbl' ; enumcur := ecur' |}) →
-    minv I m'.
-  Proof.
-    set (Σ' := #[invΣ; gen_heapΣ LAddr LWord; gen_heapΣ RegName LWord;
-                na_invΣ; sealStorePreΣ; EnclavesAgreePreΣ; EnclavesExclPreΣ; ECPreΣ; Σ]).
-    intros.
-    eapply (@template_adequacy' Σ'); eauto ; typeclasses eauto.
-  Qed.
-
-End with_adv_and_link.
-
-From cap_machine Require Import assert.
-Module assert_lib.
-Include with_adv_and_link.
-Record assert_library `{MachineParameters} := MkAssertLibrary {
-  (* assert library *)
-  assert_start : Addr;
-  assert_cap : Addr;
-  assert_flag : Addr;
-  assert_end : Addr;
-
-  assert_code_size :
-    (assert_start + length assert_subroutine_instrs)%a = Some assert_cap;
-  assert_cap_size :
-    (assert_cap + 1)%a = Some assert_flag;
-  assert_flag_size :
-    (assert_flag + 1)%a = Some assert_end;
-}.
-
-(* assert library entry *)
-Definition assert_library_content `{MachineParameters} (layout : assert_library) : gmap Addr Word :=
-  (* code for the assert subroutine, followed by a capability to the assert flag
-     and the flag itself, initialized to 0. *)
-  mkregion (assert_start layout) (assert_cap layout) (lword_get_word <$> assert_subroutine_instrs)
-  ∪ list_to_map [(assert_cap layout, WCap RW (assert_flag layout) (assert_end layout) (assert_flag layout))]
-  ∪ list_to_map [(assert_flag layout, WInt 0)] (* assert flag *).
-
-Definition lib_entry_assert `{MachineParameters} (layout : assert_library) : lib_entry :=
-  {| lib_start := assert_start layout;
-     lib_end := assert_end layout;
-     lib_entrypoint := assert_start layout;
-     lib_full_content := assert_library_content layout |}.
-
-(* full library *)
-Definition library `{MachineParameters} (layout : assert_library) : lib :=
-  {| priv_libs := [lib_entry_assert layout] ;
-     pub_libs := [] |}.
-
-Definition OK_invariant `{MachineParameters} (layout : assert_library) (m : gmap Addr Word) : Prop :=
-  ∀ w, m !! (assert_flag layout) = Some w → w = WInt 0%Z.
-
-Definition OK_dom `{MachineParameters} (layout : assert_library) : gset Addr := {[ assert_flag layout ]}.
-
-Program Definition OK_dom_correct `{MachineParameters} (layout : assert_library) :
-  ∀ m m',
-    (∀ a, a ∈ OK_dom layout → ∃ x, m !! a = Some x ∧ m' !! a = Some x) →
-    OK_invariant layout m ↔ OK_invariant layout m'.
+  rtc erased_step
+    ([Seq (Instr Executable)] , {| reg := reg ; mem := m ; etable := ∅ ; enumcur := 0%nat |})
+    (es, {| reg := reg' ; mem := m' ; etable := etbl' ; enumcur := ecur' |}) →
+  minv I m'.
 Proof.
-  intros m m' Hdom.
-  destruct Hdom with (assert_flag layout) as [w [Hw1 Hw2] ]. rewrite /OK_dom. set_solver.
-  split;intros HOK;intros w' Hw';simplify_eq;apply HOK;auto.
-Defined.
-
-Definition flag_inv `{MachineParameters} (layout : assert_library) : memory_inv :=
-  {| minv := OK_invariant layout;
-     minv_dom := {[ assert_flag layout ]} ;
-     minv_dom_correct := OK_dom_correct layout |}.
-
-Lemma flag_inv_is_initial_memory `{MachineParameters} (layout : assert_library) trusted_prog adv_prog trusted_table adv_table m :
-  is_initial_memory trusted_prog adv_prog (library layout) trusted_table adv_table m →
-  minv (flag_inv layout) m.
-Proof.
-  intros Hinit. intros a Hin.
-  destruct Hinit as (?&?&Hlibs&?&?&?&Hlibdisj).
-  cbn in Hlibs. rewrite map_union_empty in Hlibs.
-  assert ((assert_library_content layout) ⊆ m) as Hassert by auto.
-  pose proof (assert_code_size layout). pose proof (assert_cap_size layout).
-  pose proof (assert_flag_size layout).
-  assert (list_to_map [(assert_flag layout, WInt 0)] ⊆ m) as Hassert_flag.
-  { etrans;[|eauto]. eapply map_union_subseteq_r'. 2: done.
-    disjoint_map_to_list.
-    apply elem_of_disjoint. intro. rewrite elem_of_app !elem_of_finz_seq_between !elem_of_list_singleton.
-    intros [ [? ?]|?] ->; solve_addr. }
-  eapply (lookup_weaken _ _ (assert_flag layout) (WInt 0)) in Hassert_flag.
-    by simplify_eq. by simplify_map_eq.
+  set (Σ' := #[invΣ; gen_heapΣ LAddr LWord; gen_heapΣ RegName LWord;
+               na_invΣ; sealStorePreΣ; EnclavesAgreePreΣ; EnclavesExclPreΣ; ECPreΣ; Σ]).
+  intros.
+  eapply (@template_adequacy' Σ'); eauto; typeclasses eauto.
 Qed.
-
-Lemma flag_inv_sub `{MachineParameters} (layout : assert_library) :
-  minv_dom (flag_inv layout) ⊆ dom (lib_region (priv_libs (library layout))).
-Proof.
-  cbn. rewrite map_union_empty.
-  intros ? Hinit. rewrite elem_of_singleton in Hinit.
-  rewrite /assert_library_content.
-  pose proof (assert_code_size layout). pose proof (assert_cap_size layout).
-  pose proof (assert_flag_size layout).
-  rewrite /= dom_union_L. apply elem_of_union_r.
-  rewrite dom_insert_L. set_solver.
-Qed.
-
-Definition assertInv `{ceriseG Σ, MachineParameters} (layout : assert_library) :=
-  assert_inv (assert_start layout) (assert_flag layout) (assert_end layout).
-
-Definition assertN : namespace := nroot .@ "priv" .@ "assert".
-
-
-Theorem assert_template_adequacy
-  `{MP: MachineParameters} (Σ : gFunctor)
-  (layout: assert_library)
-  (P Adv: prog)
-  (P_tbl : @tbl_priv P (library layout))
-  (Adv_tbl : @tbl_pub Adv (library layout)) (r_adv : RegName)
-  (m m': Mem) (reg reg': Reg)
-  (etbl' : ETable) (ecur' : ENum)
-  (es: list cap_lang.expr):
-  let vinit := 0 in
-
-  is_initial_memory P Adv (library layout) P_tbl Adv_tbl m →
-  is_complete_memory m →
-  is_initial_registers P Adv (library layout) P_tbl Adv_tbl reg r_adv →
-  is_complete_registers reg m →
-
-  Forall (fun w => adv_condition Adv w vinit) (prog_instrs Adv) →
-
-  let filtered_map := λ (m : gmap Addr Word), filter (fun '(a, _) => a ∉ minv_dom (flag_inv layout)) m in
-  (∀ `{ceriseG Σ',sealStoreG Σ',logrel_na_invs Σ',subG Σ Σ',ReservedAddresses} (rmap : gmap RegName Word),
-      dom rmap = all_registers_s ∖ {[ PC; r_adv ]} ->
-      ⊢
-        inv invN (minv_sep (flag_inv layout) vinit)
-        ∗ na_inv logrel_nais assertN (assertInv layout vinit)
-        ∗ na_own logrel_nais ⊤
-       (* Registers *)
-       ∗ PC ↦ᵣ LCap RWX (prog_lower_bound P_tbl) (prog_end P) (prog_start P) vinit
-       ∗ r_adv ↦ᵣ LCap RWX (prog_lower_bound Adv_tbl) (prog_end Adv) (prog_start Adv) vinit
-       ∗ ([∗ map] r↦w ∈ (register_to_lregister rmap vinit), r ↦ᵣ w ∗ ⌜is_zL w = true⌝)
-       (* Memory *)
-       (* P program and table *)
-       ∗ (prog_lower_bound P_tbl, vinit) ↦ₐ (LCap RO (tbl_start P_tbl) (tbl_end P_tbl) (tbl_start P_tbl) vinit)
-       ∗ ([∗ map] a↦w ∈ (memory_to_lmemory (tbl_region P_tbl) vinit), a ↦ₐ w)
-       ∗ ([∗ map] a↦w ∈ (memory_to_lmemory (prog_region P) vinit), a ↦ₐ w)
-       (* Adv program and table *)
-       ∗ (prog_lower_bound Adv_tbl, vinit) ↦ₐ (LCap RO (tbl_start Adv_tbl) (tbl_end Adv_tbl) (tbl_start Adv_tbl) vinit)
-       ∗ ([∗ map] a↦w ∈ (memory_to_lmemory (tbl_region Adv_tbl) vinit), a ↦ₐ w)
-       ∗ ([∗ map] a↦w ∈ (memory_to_lmemory (prog_region Adv) vinit), a ↦ₐ w)
-       ∗ EC⤇ 0
-       ∗ ([∗ set] o ∈ gset_all_otypes, can_alloc_pred o)
-
-        -∗ WP Seq (Instr Executable) {{ λ _, True }}) →
-
-    rtc erased_step
-      ([Seq (Instr Executable)] , {| reg := reg ; mem := m ; etable := ∅ ; enumcur := 0 |})
-      (es, {| reg := reg' ; mem := m' ; etable := etbl' ; enumcur := ecur' |}) →
-  minv (flag_inv layout) m'.
-Proof.
-  intros ? ? ? ? ? ? ? Hspec.
-  eapply (template_adequacy Σ);[eauto..|]; (* rewrite /invGpreS. solve_inG. *)
-    try typeclasses eauto.
-  { eapply flag_inv_is_initial_memory;eauto. }
-  { eapply flag_inv_sub;eauto. }
-  intros. cbn.
-  rewrite !map_union_empty.
-  iIntros "(#Hflag & Hown & HPC & Hr_adv & Hrmap & Htbl & Htbl_r
-           & Hprog & Htbl_adv & Htbl_adv_r & Hprog_adv & _ & Hassert & HEC & Hseal_store)".
-
-  (* allocate the flag invariant *)
-  iMod (na_inv_alloc logrel_nais ⊤ assertN (assertInv layout vinit)
-          with "[Hassert]") as "#Hinv_assert".
-  { iNext. rewrite /assertInv /assert_inv /assert_library_content.
-    iExists (assert_cap layout).
-    pose proof (assert_code_size layout). pose proof (assert_cap_size layout).
-    pose proof (assert_flag_size layout).
-    rewrite map_filter_union.
-    2: { disjoint_map_to_list. apply elem_of_disjoint. intro.
-         rewrite elem_of_app elem_of_finz_seq_between !elem_of_list_singleton.
-         intros [ [? ?]|?]; solve_addr. }
-    rewrite memory_to_lmemory_union.
-    iDestruct (big_sepM_union with "Hassert") as "[Hassert _]".
-    { apply memory_to_lmemory_disjoint.
-      eapply map_disjoint_filter. disjoint_map_to_list.
-      apply elem_of_disjoint. intro.
-      rewrite elem_of_app elem_of_finz_seq_between !elem_of_list_singleton.
-      intros [ [? ?]|?]; solve_addr. }
-    rewrite map_filter_id.
-    2: { intros ? ? HH%elem_of_dom_2. rewrite !dom_union_L dom_mkregion_eq in HH.
-         2: solve_addr. apply elem_of_union in HH.
-         rewrite elem_of_singleton. destruct HH as [HH|HH].
-         rewrite -> elem_of_list_to_set, elem_of_finz_seq_between in HH; solve_addr.
-         rewrite -> dom_list_to_map_singleton, elem_of_list_to_set, elem_of_list_singleton in HH; solve_addr. }
-    rewrite memory_to_lmemory_union.
-    iDestruct (big_sepM_union with "Hassert") as "[Hassert Hcap]".
-    { apply memory_to_lmemory_disjoint.
-      disjoint_map_to_list. apply elem_of_disjoint. intro.
-      rewrite elem_of_finz_seq_between !elem_of_list_singleton. solve_addr. }
-    subst vinit.
-    rewrite memory_to_lmemory_insert.
-    iEval (cbn) in "Hcap".
-    iDestruct (big_sepM_insert with "Hcap") as "[Hcap _]"; first done.
-    iFrame "Hcap".
-    iSplitL "Hassert"; cycle 1.
-    + iPureIntro. repeat split; solve_addr.
-    + iApply (mkregion_sepM_to_sepL2 with "[Hassert]"); auto.
-      { apply Forall_forall.
-        intros.
-        cbn in *.
-        repeat (rewrite elem_of_cons in H12; destruct H12 as [-> | H12]; first done).
-        set_solver+H12.
-      }
-      { solve_addr. }
-      rewrite (_: assert_cap layout = assert_start layout ^+ length assert_subroutine_instrs)%a. 2: solve_addr.
-    iFrame "Hassert".
-    }
-
-  iApply Hspec; [exact|..|iFrame "∗ #"];auto.
-Qed.
-
-End assert_lib.
