theories/examples/enclaves/trusted_compute_adequacy.v
@@ -1,11 +1,3 @@
-(* From iris.algebra Require Import frac. *)
-(* From iris.proofmode Require Import proofmode. *)
-(* Require Import Eqdep_dec List. *)
-(* From cap_machine Require Import rules seal_store. *)
-(* From cap_machine Require Import logrel fundamental. *)
-(* From cap_machine Require Import proofmode. *)
-(* From cap_machine Require Import macros_new. *)
-(* Open Scope Z_scope. *)
 From iris.proofmode Require Import proofmode.
 From cap_machine Require Import rules logrel fundamental.
 From cap_machine Require Import proofmode.
@@ -16,33 +8,24 @@ From cap_machine Require Import
   trusted_compute_enclave_spec
   trusted_compute_spec
 .
-(* From cap_machine Require Import attestation_adequacy_template. *)
 
-(* Instance DisjointList_list_Addr : DisjointList (list Addr). *)
-(* Proof. exact (@disjoint_list_default _ _ app []). Defined. *)
-
-Import assert_lib.
 Class memory_layout `{MachineParameters} := {
   (* Verifier code *)
-  verifier_region_start : Addr;
   verifier_start : Addr;
   verifier_end : Addr;
   verifier_size: (verifier_start + trusted_compute_main_len = Some verifier_end)%a;
-  verifier_region_start_offset: (verifier_region_start + 0)%a = Some verifier_start;
   verifier_region: list Addr;
   verifier_region_correct:
-    verifier_region = (finz.seq_between verifier_region_start verifier_end);
+    verifier_region = (finz.seq_between verifier_start verifier_end);
 
   (* Adversary code *)
-  adv_region_start : Addr;
   adv_start : Addr;
   adv_end : Addr;
   adv_instrs : list Word;
   adv_size : (adv_start + (length adv_instrs) = Some adv_end)%a ;
-  adv_region_start_offset: (adv_region_start + 0)%a = Some adv_start;
   adv_region: list Addr;
   adv_region_correct:
-    adv_region = (finz.seq_between adv_region_start adv_end);
+    adv_region = (finz.seq_between adv_start adv_end);
 
   (* Assert routine *)
   l_assert_start : Addr;
@@ -87,8 +70,11 @@ Class memory_layout `{MachineParameters} := {
 Local Instance trusted_compute_concrete `{memory_layout} : TrustedCompute.
 Proof. apply (Build_TrustedCompute tc_enclave_start). Defined.
 
+Definition link_tbl_cap `{memory_layout} :=
+ WCap RO link_table_start link_table_end link_table_start.
+
 Program Definition tc_verifier_prog `{memory_layout} : prog :=
-  let link_cap := WCap RO link_table_start link_table_end link_table_start in
+  let link_cap := link_tbl_cap in
   let a_data := (verifier_start ^+ trusted_compute_main_code_len)%a in
   let data_cap := WCap RWX verifier_start verifier_end a_data  in
   {| prog_start := verifier_start ;
@@ -111,7 +97,7 @@ Definition adv_prog `{memory_layout} : prog :=
      prog_instrs := adv_instrs ;
      prog_size := adv_size |}.
 
-Program Definition layout `{memory_layout} : assert_library :=
+Program Definition assert_layout `{memory_layout} : assert_library :=
   {| (* assertion fail library *)
      assert_start := l_assert_start;
      assert_cap := l_assert_cap;
@@ -122,34 +108,311 @@ Program Definition layout `{memory_layout} : assert_library :=
      assert_cap_size := l_assert_cap_size;
      assert_flag_size := l_assert_flag_size;
   |}.
-Definition AssertLibrary `{memory_layout} := library layout.
 
-(* Program Definition tc_link_table `{memory_layout} : @tbl_priv tc_verifier_prog AssertLibrary := *)
-(*   {| prog_lower_bound := verifier_region_start ; *)
-(*      tbl_start := link_table_start ; *)
-(*      tbl_end := link_table_end ; *)
-(*      tbl_size := link_table_size ; *)
-(*      tbl_prog_link := verifier_region_start_offset ; *)
-(*      tbl_disj := _ *)
-(*   |}. *)
-(* Next Obligation. *)
-(*   intros. simpl. *)
-(*   pose proof (regions_disjoint) as Hdisjoint. *)
-(*   rewrite !disjoint_list_cons in Hdisjoint |- *. *)
-(*   disjoint_map_to_list. set_solver. *)
-(* Qed. *)
 
-(* Program Definition adv_table `{memory_layout} : @tbl_pub adv_prog AssertLibrary := *)
-(*   {| prog_lower_bound := adv_region_start ; *)
-(*      tbl_start := adv_link_table_start ; *)
-(*      tbl_end := adv_link_table_end ; *)
-(*      tbl_size := adv_link_table_size ; *)
-(*      tbl_prog_link := adv_region_start_offset ; *)
-(*      tbl_disj := _ *)
-(*   |}. *)
-(* Next Obligation. *)
-(*   intros. simpl. *)
-(*   pose proof (regions_disjoint) as Hdisjoint. *)
-(*   rewrite !disjoint_list_cons in Hdisjoint |- *. *)
-(*   disjoint_map_to_list. set_solver. *)
-(* Qed. *)
+Definition tbl_assert_tbl `{memory_layout} : assert_tbl :=
+  {|
+    tbl_start := link_table_start;
+    tbl_end :=link_table_end;
+    tbl_size := link_table_size;
+  |}.
+
+Section tc_adequacy.
+  Context {Σ:gFunctors}
+          `{MP: MachineParameters}
+          {ceriseg:ceriseG Σ} {sealsg: sealStoreG Σ}
+          {nainv: logrel_na_invs Σ}
+          {memlayout: memory_layout}
+  .
+
+  Definition link_tableN := (trusted_computeN.@"link_table").
+  Definition tc_mainN := (trusted_computeN.@"main").
+  Lemma tc_correct :
+    let vinit := 0%nat in
+    let P := tc_verifier_prog in
+    let Adv := adv_prog in
+    let AssertLib := assert_layout in
+    let RA := reserved_addresses_assert AssertLib vinit in
+    let r_adv := r_t0 in
+
+    finz.seq_between adv_start adv_end ## reserved_addresses ->
+    Forall (λ w, is_z w = true \/ in_region w adv_start adv_end) adv_instrs →
+    let filtered_map := λ (m : gmap Addr Word), filter (fun '(a, _) => a ∉ minv_dom (adequacy_flag_inv AssertLib)) m in
+    (∀ rmap,
+      dom rmap = all_registers_s ∖ {[ PC; r_adv ]} →
+     ⊢ inv invN (minv_sep (adequacy_flag_inv AssertLib) vinit)
+     ∗ na_inv logrel_nais assertN (assertInv AssertLib vinit)
+     ∗ na_own logrel_nais ⊤ (*XXX*)
+
+     (* Registers *)
+     ∗ PC ↦ᵣ LCap RWX (prog_start P) (prog_end P) (prog_start P) vinit
+     ∗ r_adv ↦ᵣ LCap RWX (prog_start Adv) (prog_end Adv) (prog_start Adv) vinit
+     ∗ ([∗ map] r↦w ∈ (register_to_lregister rmap vinit), r ↦ᵣ w ∗ ⌜is_zL w = true⌝)
+
+     (* Memory *)
+     (* P program *)
+     ∗ ([∗ map] a↦w ∈ (memory_to_lmemory (prog_region P) vinit), a ↦ₐ w)
+     (* Adv program  *)
+     ∗ ([∗ map] a↦w ∈ (memory_to_lmemory (prog_region Adv) vinit), a ↦ₐ w)
+     (* Linking Table *)
+     ∗ ([∗ map] a↦w ∈ (memory_to_lmemory (assert_tbl_region tbl_assert_tbl AssertLib) vinit), a ↦ₐ w)
+
+     ∗ EC⤇ 0%nat
+     ∗ ([∗ set] o ∈ gset_all_otypes, can_alloc_pred o)
+
+        -∗ WP Seq (Instr Executable) {{ λ _, True }}).
+  Proof.
+    intros *.
+    iIntros (Hreserved Hints Hfilter rmap Hdom)
+      "(#Hinv & #Hassert & Hown & HPC & Hr_adv & Hrmap & Hprog & Hadv & Hlink & HEC & Hseal_store)".
+
+    simpl.
+    iMod ( custom_enclaves_inv_alloc (enclaves_map := contract_tc_enclaves_map) with
+           "[$HEC $Hseal_store]") as "#Hsystem_inv".
+
+    iMod (na_inv_alloc logrel_nais ⊤ link_tableN
+            (((tbl_start tbl_assert_tbl), vinit) ↦ₐ word_to_lword (assert_entry_point AssertLib) vinit)
+           with "[Hlink]") as "#Hinv_link".
+    { iNext.
+    rewrite /assert_tbl_region.
+    rewrite /mkregion.
+    cbn.
+    rewrite finz_seq_between_cons.
+    2:{ pose proof link_table_size as H; solve_addr + H. }
+    rewrite finz_seq_between_empty.
+    2:{ pose proof link_table_size as H; solve_addr + H. }
+    cbn.
+    rewrite memory_to_lmemory_insert /=.
+    iDestruct (big_sepM_insert_delete with "Hlink") as "[$ _]".
+    }
+
+    (* allocate validity of adversary *)
+    iAssert (|={⊤}=> interp (LCap RWX adv_start adv_end adv_start vinit))%I with "[Hadv]" as ">#Hadv".
+    {
+      pose proof adv_size as Hadv_size'.
+      iApply (region_valid_in_regionL _ _ _ _ _ ((fun w=> word_to_lword w vinit) <$> adv_instrs));auto.
+      - apply Forall_forall. intros. set_solver+.
+      - apply Forall_forall. intros.
+        rewrite Forall_forall in Hints.
+        apply elem_of_list_fmap_2 in H.
+        destruct H as (w & -> & Hw).
+        specialize (Hints w Hw).
+        destruct Hints.
+        + left. destruct w ; cbn in * ; done.
+        + right.
+          rewrite /in_regionL.
+          rewrite /in_region in H.
+          destruct w ; cbn in * ; try done.
+          destruct sb ; cbn in * ; try done.
+          naive_solver.
+      - iApply (big_sepM_to_big_sepL2 with "[Hadv]").
+        + apply finz_seq_between_NoDup.
+        + rewrite fmap_length.
+          rewrite finz_seq_between_length /finz.dist /=. solve_addr+Hadv_size'.
+        + subst Adv ; cbn.
+          rewrite /prog_region /adv_prog; cbn.
+          rewrite memory_to_lmemory_mk_logical_region_map.
+          rewrite /logical_region_map.
+          rewrite -logical_region_map_list_to_map; first done.
+          * apply finz_seq_between_NoDup.
+          * rewrite fmap_length.
+            rewrite finz_seq_between_length /finz.dist /=. solve_addr+Hadv_size'.
+    }
+
+    set (a_data := (prog_start P ^+ length (trusted_compute_main_code 0))%a).
+    set (link_cap := word_to_lword link_tbl_cap vinit).
+    iMod (na_inv_alloc logrel_nais ⊤ tc_mainN
+           (codefrag (prog_start P) vinit (trusted_compute_main_code 0)
+            ∗ (a_data, vinit) ↦ₐ link_cap
+            ∗ ((a_data ^+ 1)%a, vinit) ↦ₐ LCap RWX (prog_start P) (prog_end P) a_data vinit)
+         with "[Hprog]") as "#Hprog".
+    { iNext.
+      replace (prog_region P)
+        with
+        (mkregion verifier_start verifier_end
+                 ((lword_get_word <$> trusted_compute_main_code 0) ++
+                 [link_tbl_cap;
+                  WCap RWX verifier_start verifier_end (verifier_start ^+ trusted_compute_main_code_len)%a])
+              ) by done.
+      pose proof verifier_size as Hsize_verifier.
+      rewrite /trusted_compute_main_len in Hsize_verifier.
+      rewrite mkregion_app; last done.
+      rewrite memory_to_lmemory_union.
+      iDestruct (big_sepM_union with "Hprog") as "[Hprog Hdata]".
+      { apply memory_to_lmemory_disjoint.
+        rewrite /mkregion.
+        apply map_disjoint_list_to_map_zip_l.
+        + rewrite fmap_length.
+          rewrite finz_seq_between_length.
+          apply finz_dist_add.
+          exists (verifier_start ^+ length (trusted_compute_main_code 0))%a.
+          cbn in *.
+          solve_addr.
+        + apply Forall_forall.
+          intros a Ha.
+          apply not_elem_of_list_to_map.
+          rewrite fst_zip.
+          * rewrite elem_of_finz_seq_between in Ha.
+            rewrite not_elem_of_finz_seq_between.
+            solve_addr.
+          * rewrite fmap_length.
+            rewrite finz_seq_between_length.
+            cbn.
+            rewrite finz_dist_S; last solve_addr.
+            rewrite finz_dist_S; last solve_addr.
+            rewrite finz_dist_0; last solve_addr.
+            done.
+      }
+
+      replace ([link_tbl_cap; WCap RWX verifier_start verifier_end (verifier_start ^+ trusted_compute_main_code_len)%a])
+        with ([link_tbl_cap]++[WCap RWX verifier_start verifier_end
+                                 (verifier_start ^+ trusted_compute_main_code_len)%a]); last by cbn.
+      rewrite mkregion_app; last solve_addr.
+      rewrite memory_to_lmemory_union.
+      iDestruct (big_sepM_union with "Hdata") as "[Hdata1 Hdata2]".
+      { apply memory_to_lmemory_disjoint.
+        rewrite /mkregion.
+        apply map_disjoint_list_to_map_zip_l.
+        + rewrite finz_seq_between_length.
+          apply finz_dist_add.
+          exists (verifier_start ^+ 38)%a.
+          cbn in *.
+          solve_addr.
+        + apply Forall_forall.
+          intros a Ha.
+          apply not_elem_of_list_to_map.
+          rewrite fst_zip.
+          * rewrite elem_of_finz_seq_between in Ha.
+            rewrite not_elem_of_finz_seq_between.
+            solve_addr.
+          * rewrite finz_seq_between_length.
+            cbn.
+            rewrite finz_dist_S; last solve_addr.
+            rewrite finz_dist_0; last solve_addr.
+            done.
+      }
+
+      iSplitL "Hprog"; [|iSplitL "Hdata1"].
+      - rewrite /codefrag /region_mapsto.
+        iApply (big_sepM_to_big_sepL2 with "[Hprog]").
+        { apply NoDup_fmap; first (intros ? ? ?; by simplify_eq).
+          apply finz_seq_between_NoDup.
+        }
+        { rewrite fmap_length.
+          rewrite finz_seq_between_length.
+          cbn.
+          apply finz_dist_add.
+          exists (verifier_start ^+ 37%nat)%a.
+          solve_addr.
+        }
+        iEval (rewrite memory_to_lmemory_mk_logical_region_map) in "Hprog".
+        iFrame.
+      - iEval (rewrite memory_to_lmemory_mk_logical_region_map) in "Hdata1".
+        rewrite finz_seq_between_cons; last solve_addr.
+        rewrite finz_seq_between_empty; last solve_addr.
+        iDestruct (big_sepM_insert_delete with "Hdata1") as "[$ _]".
+      - iEval (rewrite memory_to_lmemory_mk_logical_region_map) in "Hdata2".
+        rewrite finz_seq_between_cons; last solve_addr.
+        rewrite finz_seq_between_empty; last solve_addr.
+        iDestruct (big_sepM_insert_delete with "Hdata2") as "[$ _]".
+    }
+
+    iAssert (tc_main_inv verifier_start verifier_end vinit (trusted_compute_main_code 0) a_data
+               link_cap tc_mainN) with "Hprog" as "#Hprog_inv".
+    iAssert (assert_inv (assert_start AssertLib) (assert_flag AssertLib) (assert_end AssertLib)
+               vinit assertN)
+      with "Hassert" as "Hassert_inv".
+
+    iAssert (flag_inv (assert_flag AssertLib) vinit invN) with "[Hinv]" as
+      "#Hflag_inv".
+    { iApply (inv_iff with "Hinv []").
+      iNext. iModIntro.
+      iSplit.
+      - rewrite /minv_sep /=. iIntros "HH". iDestruct "HH" as (m) "(Hm & %Heq & %HOK)".
+        assert (is_Some (m !! l_assert_flag)) as [? Hlook].
+        { apply elem_of_dom. rewrite Heq. apply elem_of_singleton. auto. }
+        assert ( (memory_to_lmemory m vinit) !! (l_assert_flag, vinit) = Some (word_to_lword x vinit)) as Hlook_log.
+        { rewrite memory_to_lmemory_lookup.
+          by rewrite Hlook; cbn.
+        }
+        iDestruct (big_sepM_lookup _ _ (l_assert_flag,vinit) with "Hm") as "Hflag"; eauto.
+        apply HOK in Hlook as ->.
+        iFrame.
+      - iIntros "HH". iExists {[ l_assert_flag := WInt 0%Z ]}.
+        rewrite /memory_to_lmemory map_fmap_singleton kmap_singleton.
+        rewrite big_sepM_singleton. iFrame.
+        rewrite dom_singleton_L /minv_dom /=. iSplit;auto.
+        rewrite /OK_invariant. iPureIntro. intros w Hw. simplify_map_eq. done.
+    }
+
+    pose proof ( verifier_size ) as Hverifier_size.
+    replace verifier_end with (verifier_start ^+ trusted_compute_main_len)%a by solve_addr.
+
+    iApply (wp_wand with "[-]").
+    - iApply (trusted_compute_full_run_spec with
+      "[$Hadv $Hsystem_inv $Hinv_link $Hassert $Hprog_inv $Hflag_inv ] [ $HPC $Hown $Hr_adv $Hrmap]"); auto.
+      + solve_ndisj.
+      + solve_ndisj.
+      + solve_ndisj.
+      + subst P; rewrite /tc_verifier_prog /=.
+        solve_addr.
+      + rewrite /SubBounds.
+        split; first solve_addr.
+        split; last solve_addr.
+        subst P; rewrite /tc_verifier_prog /=.
+        rewrite /trusted_compute_main_len.
+        solve_addr.
+      + pose proof link_table_size.
+        cbn; solve_addr.
+      + pose proof link_table_size.
+        cbn.
+        apply le_addr_withinBounds; solve_addr.
+      + rewrite /register_to_lregister.
+        by rewrite dom_fmap_L.
+    - by iIntros (v) "H".
+  Qed.
+
+End tc_adequacy.
+
+
+Theorem tc_enclaves_adequacy `{memory_layout}
+    (m m': Mem) (reg reg': Reg) (etbl' : ETable) (ecur' : ENum)
+    (es: list cap_lang.expr):
+  is_initial_memory tc_verifier_prog adv_prog assert_layout tbl_assert_tbl m →
+  is_complete_memory m →
+  is_initial_registers tc_verifier_prog adv_prog assert_layout tbl_assert_tbl reg r_t0 →
+  is_complete_registers reg m →
+  Forall (λ w, is_z w = true \/ in_region w adv_start adv_end) (prog_instrs adv_prog) →
+
+  rtc erased_step ([Seq (Instr Executable)] , {| reg := reg ; mem := m ; etable := ∅ ; enumcur := 0%nat |})
+    (es, {| reg := reg' ; mem := m' ; etable := etbl' ; enumcur := ecur' |}) →
+  (∀ w, m' !! l_assert_flag = Some w → w = WInt 0%Z).
+Proof.
+  intros ? ? ? ? Hints.
+  set (Σ' := #[]).
+  pose proof (template_adequacy Σ' tc_verifier_prog adv_prog assert_layout tbl_assert_tbl) as Hadequacy.
+  eapply Hadequacy;eauto.
+  - eapply adequacy_flag_inv_is_initial_memory; eauto.
+  - intros Σ ? ? ? ? ? ?.
+    iIntros "(?&?&?&?&?&?&?&?&?&?&?)".
+    iApply tc_correct; eauto; last iFrame.
+
+    cbn.
+    clear.
+    pose proof regions_disjoints as (_&_&_&Hdisj&_).
+    rewrite adv_region_correct in Hdisj.
+    rewrite l_assert_region_correct in Hdisj.
+    rewrite elem_of_disjoint.
+    intros a Ha Ha'.
+
+    rewrite elem_of_disjoint in Hdisj.
+    eapply Hdisj; eauto.
+    rewrite elem_of_finz_seq_between.
+    rewrite elem_of_list_singleton in Ha'; simplify_eq.
+
+    pose proof l_assert_code_size.
+    pose proof l_assert_cap_size.
+    pose proof l_assert_flag_size.
+
+    solve_addr.
+Qed.
